Restore reachability analysis.

theories/Reachability/ReachabilityAnalysis.v
@@ -2,7 +2,7 @@ Require Import CSet Le Var.
 
 Require Import Plus Util AllInRel Map CSet ListUpdateAt.
 Require Import Val Var Env IL Annotation Infra.Lattice DecSolve Filter.
-Require Import Analysis AnalysisForwardSSA FiniteFixpointIteration Terminating Subterm.
+Require Import Analysis AnalysisForward FiniteFixpointIteration Terminating Subterm.
 
 Remove Hints trans_eq_bool.
 
@@ -11,32 +11,33 @@ Set Implicit Arguments.
 Definition reachability_transform (sT:stmt)
            (ZL:list params)
            (st:stmt) (ST:subTerm st sT)
-           (ZLIncl:list_union (of_list ⊝ ZL) [<=] occurVars sT) (u:unit)
            (d:bool)
-  : anni unit st :=
+  : anni bool :=
   match st with
+  | stmtLet x e s => anni1 d
   | stmtIf e s t =>
-    (if [op2bool e = Some false] then false else d,
-     if [op2bool e = Some true] then false else d, u)
-  | _ => u
+    anni2 (if [op2bool e = Some false] then false else d)
+          (if [op2bool e = Some true] then false else d)
+  | stmtApp f Y => anni1 d
+  | stmtReturn e => anni1 d
+  | _ => anni1 d
   end.
 
+
 Lemma reachability_transform_monotone (sT s : stmt) (ST : subTerm s sT)
-      (ZL : 〔params〕) (ZLIncl : list_union (of_list ⊝ ZL) [<=] occurVars sT) (a b : unit)
+      (ZL : 〔params〕) (a b : bool)
   : a ⊑ b
-    ->  forall r r' : bool,
-      r ⊑ r'
-      -> reachability_transform ZL ST ZLIncl a r ⊑ reachability_transform ZL ST ZLIncl b r'.
+    -> reachability_transform ZL ST a ⊑ reachability_transform ZL ST b.
 Proof.
   intros; destruct s; simpl; try econstructor; simpl; eauto;
     repeat cases; simpl in *; eauto.
 Qed.
 
 Definition reachability_analysis s :=
-  makeForwardAnalysis (fun s => unit ) _ _
+  makeForwardAnalysis (fun s => bool ) _ _ _
                       reachability_transform
                       reachability_transform_monotone
-                      (fun s => Terminating_unit) s.
+                      (fun s => terminating_bool) s true.
 
 Definition reachabilityAnalysis s :=
-  proj1_sig (safeFixpoint (reachability_analysis s)).
+  proj1_sig (proj1_sig (safeFixpoint (reachability_analysis s))).
