theories/Reachability/ReachabilityAnalysisCorrect.v
@@ -1,23 +1,22 @@
 Require Import CSet Le Var.
 
 Require Import Plus Util AllInRel Map CSet OptionR MoreList.
-Require Import Val Var Env IL Annotation Infra.Lattice RenamedApart.
+Require Import Val Var Env IL Annotation Infra.Lattice.
 Require Import DecSolve Analysis Filter Terminating.
-Require Import Analysis AnalysisForwardSSA FiniteFixpointIteration.
-Require Import Reachability Subterm AnnotationLattice DomainSSA.
+Require Import Analysis AnalysisForward FiniteFixpointIteration.
+Require Import Reachability ReachabilityAnalysis Subterm.
 
 Set Implicit Arguments.
 
 Local Arguments proj1_sig {A} {P} e.
 Local Arguments length {A} e.
-Local Arguments forward {sT} {D} {H} {H0} exp_transf reach_transf ZL ZLIncl st ST d anr.
+Local Arguments forward {sT} {Dom} {H} {H0} {H1} ftransform ZL st ST d a.
 
 Opaque poLe.
 
 (* Coq can't figure out the instantiation (fun _ => bool) via unification,
    so we have to add this specialized lemma *)
-
-(*Lemma forward_length_ass_UC
+Lemma forward_length_ass_UC
       (sT : stmt)
       (f : forall sT0 : stmt,
           〔params〕 ->
@@ -29,570 +28,126 @@ Opaque poLe.
 Qed.
 
 Hint Resolve forward_length_ass_UC.
- *)
 
-Lemma poEq_pair_inv A `{PartialOrder A} B `{PartialOrder B} (x y:A * B)
-  : poEq x y <-> poEq (fst x) (fst y) /\ poEq (snd x) (snd y).
+Definition reachability_sound sT ZL BL s d a (ST:subTerm s sT)
+  : poEq (fst (forward reachability_transform ZL s ST d a)) a
+    -> annotation s a
+    -> labelsDefined s (length ZL)
+    -> labelsDefined s (length BL)
+    -> poLe (snd (@forward sT _ _ _ _ reachability_transform ZL s ST d a)) BL
+    -> reachability cop2bool Sound BL s a.
 Proof.
-  firstorder.
-Qed.
-
-Smpl Add 120
-     match goal with
-     | [ H : poEq (_,_) (_,_) |- _ ] =>
-       rewrite poEq_pair_inv in H; simpl fst in H; simpl snd in H;
-         let H' := fresh H in destruct H as [H H']
-     | [H : poEq ?x ?x |- _ ] => clear H
-     end : inv_trivial.
-
-
-Ltac is_in_context X :=
-  match goal with
-  | [ H : ?Y  |- _ ] =>
-    unify X Y
-  end.
-
-Smpl Add 120 match goal with
-         | [ H : ?x = getAnn ?y, I : context [ setTopAnn ?y ?x ] |- _ ] =>
-           rewrite (@setTopAnn_eta _ _ _ (eq_sym H)) in I
-         | [ H : getAnn ?y = ?x, I : context [ setTopAnn ?y ?x ] |- _ ] =>
-           rewrite (@setTopAnn_eta _ _ _ H) in I
-         end : inv_trivial.
-
-Ltac simpl_forward_setTopAnn :=
-  match goal with
-  | [H : ann_R _ (snd (fst (@forward ?sT ?D ?PO ?JSL ?f ?fr ?ZL ?ZLIncl
-                                     ?s ?ST ?d ?r))) ?r' |- _ ] =>
-    let X := fresh "HEQ" in
-    match goal with
-    | [ H' : getAnn r = getAnn r' |- _ ] => fail 1
-    | _ => first
-            [ unify r r'; fail 1
-            | exploit (@forward_getAnn sT D PO JSL f fr ZL ZLIncl s ST d r r' H) as X;
-              subst]
-    end
-  end; subst; try eassumption;
-  try rewrite getAnn_setTopAnn in *;
-  repeat rewrite setTopAnn_eta' in *.
-
-Smpl Add 130 simpl_forward_setTopAnn : inv_trivial.
-
-
-
-Lemma domupdd_eq (D : Type) `{PartialOrder D} (U : ⦃nat⦄) (d:VDom U D) x v pf
-  : domenv (proj1_sig d) x === v
-    -> d ≣ @domupdd _ _ d x v pf.
-Proof.
-  eapply poEq_domupd; eauto.
-Qed.
-
-Opaque poEq.
-
-(*
-Lemma vdom_upd_inv sT (D : Type) `{JoinSemiLattice D} (d d':VDom (occurVars sT) D) f fr ZL ZLIncl s (ST:subTerm s sT) r (AN:annotation s r)
-      (EQ: fst (forward f fr ZL ZLIncl s ST d' r) ≣ (d,r))
-      (fExt: forall U e (a a':VDom U D), a ≣ a' -> forall b b', b ≣ b' -> f _ b a e ≣ f _ b' a' e)
-      (frExt:forall U e (a a':VDom U D),
-          a ≣ a' -> forall b b', b ≣ b' -> fr _ b a e ≣ fr _ b' a' e)
-  :  d === d'.
-Proof.
-  general induction AN; subst; simpl in *; dcr;
-    repeat let_pair_case_eq; repeat let_case_eq; repeat simpl_pair_eqs; subst; simpl in *;
-      simpl in *; clear_trivial_eqs.
-  - eapply IHAN; eauto.
-    split; simpl.
-    + etransitivity; eauto.
-      eapply forward_ext; eauto.
-      admit.
-    + Transparent poEq.
-      etransitivity; eauto.
-      eapply forward_ext; eauto.
-      eapply domupdd_eq.
-      exploit (@forward_agree sT _ _ _ f fr ZL (domupdd d' (f (occurVars sT) (getAnn sa) d' e) (subTerm_EQ_Let_x eq_refl ST)) (singleton x) s (subTerm_EQ_Let eq_refl ST) ZLIncl); eauto; dcr.
-      etransitivity. symmetry. eapply
-      eapply H2. admit.
-
-Qed.
-*)
-Opaque poEq.
-Opaque poLe.
-
-
-Ltac PIR2_eq_simpl :=
-  match goal with
-  | [ H : PIR2 (ann_R eq) _ _ |- _ ] =>
-    eapply PIR2_R_impl with (R':=eq) in H;
-    [|intros ? ?; rewrite <- ann_R_eq; let A := fresh "A" in intros A; apply A]
-  | [ H : PIR2 eq _ _ |- _ ] =>
-    eapply PIR2_eq in H
-  | [ H : ann_R eq _ _ |- _ ] => rewrite ann_R_eq in H
-  end.
-
-(*
-Definition reachability_sound_indep (sT:stmt) D `{JoinSemiLattice D}
-           f fr pr ZL BL s (d:VDom (occurVars sT) D) r (ST:subTerm s sT) ZLIncl
-           (EQ:snd (fst (forward f fr ZL ZLIncl s ST d r)) ≣ r)
-           (Ann: annotation s r)
-           (DefZL: labelsDefined s (length ZL))
-           (DefBL: labelsDefined s (length BL))
-           (BL_le: poLe (snd (forward f fr ZL ZLIncl s ST d r)) BL)
-           (fExt:forall (U : ⦃nat⦄) (e : exp) (a0 a' : VDom U D),
-               a0 ≣ a' -> forall b b' : bool, b ≣ b' -> f U b a0 e ≣ f U b' a' e)
-           (frIndep:forall U e (a a':VDom U D),
-               forall b b', b ≣ b' -> fr _ b a e ≣ fr _ b' a' e)
-  : reachability pr Sound BL s r.
-Proof.
+  intros EQ Ann DefZL DefBL.
   general induction Ann; simpl in *; inv DefZL; inv DefBL;
-    repeat let_case_eq; repeat simpl_pair_eqs; subst; simpl in *;
-      simpl in *; clear_trivial_eqs.
-  Transparent poEq.
-  - econstructor; eauto.
-  - econstructor; eauto.
-    + rewrite <- HEQ0. admit.
-    + rewrite <- HEQ. admit.
-    + eapply IHAnn1; eauto.
-      eapply @PIR2_zip_join_inv_left. eauto.
+    repeat let_case_eq; repeat simpl_pair_eqs; subst; simpl in *.
+  - inv EQ.
+    pose proof (ann_R_get H7); simpl in *.
+    econstructor; eauto.
+    simpl_forward_setTopAnn; eauto.
+  - assert (forall d d', ❬snd (forward reachability_transform ZL s (subTerm_EQ_If1 eq_refl ST) d sa)❭ =
+            ❬snd (forward reachability_transform ZL t (subTerm_EQ_If2 eq_refl ST) d' ta)❭). {
       eauto with len.
-    + eapply IHAnn2; eauto.
-      eapply @PIR2_zip_join_inv_right. eauto.
-      eauto with len.
+    }
+    repeat cases in EQ; simpl in *; try solve [congruence]; inv EQ;
+    repeat simpl_forward_setTopAnn;
+    econstructor; intros; try solve [congruence];
+      eauto using @PIR2_zip_join_inv_left, @PIR2_zip_join_inv_right; simpl; eauto.
+    exfalso. eapply H3.
+    rewrite op2bool_cop2bool in COND; eauto. rewrite COND. reflexivity.
+    exfalso. eapply H3.
+    rewrite op2bool_cop2bool in COND; eauto. rewrite COND. reflexivity.
   - edestruct get_in_range; eauto.
     edestruct get_in_range; try eapply H4; eauto.
-    Transparent poLe. hnf in BL_le.
-    edestruct PIR2_nth; eauto using ListUpdateAt.list_update_at_get_3; dcr.
-    econstructor; simpl; eauto.
-  - econstructor; eauto.
-  - set (FWt:=(forward f fr (fst ⊝ s ++ ZL) (ZLIncl_ext ZL eq_refl ST ZLIncl) t
-                       (subTerm_EQ_Fun1 eq_refl ST) d ta)) in *.
-    set (FWF:=@forwardF sT (sTDom D) (snd FWt) (forward f fr (fst ⊝ s ++ ZL) (ZLIncl_ext ZL eq_refl ST ZLIncl)) s (joinTopAnn (A:=bool) ⊜ sa (snd FWt)) (fst (fst FWt)) (subTerm_EQ_Fun2 eq_refl ST)) in *.
-    eapply PIR2_get in H16; eauto with len.
-    assert (LenA:❬s❭ <= ❬snd FWt❭). {
-      subst FWt. len_simpl. omega.
-    }
-
-    assert (LenB:❬fst ⊝ s ++ ZL❭ = ❬snd FWt❭). {
-      subst FWt. len_simpl. omega.
-    }
-    econstructor; eauto.
-    + eapply IHAnn; eauto.
-      * erewrite (take_eta ❬s❭) at 1. eapply PIR2_app; eauto.
-        -- change (PIR2 impb) with (@poLe (list bool) _).
-           assert (PIR2 impb (Take.take ❬s❭ (snd FWt)) (getAnn ⊝ sa)). {
-             change (PIR2 impb) with (PIR2 (@poLe bool _)).
-             rewrite H.
-             exploit (snd_forwardF_inv _ _ _ _ _ _ _ H16); eauto.
-             eapply (@joinTopAnn_map_inv); eauto.
-           }
-           rewrite <- H4. subst FWF.
-           subst FWt. reflexivity.
-        -- rewrite <- BL_le.
-           eapply PIR2_drop.
-           etransitivity;[| eapply forwardF_mon; eauto].
-           reflexivity.
-           subst FWt.
-           eauto with len.
-    + intros.
-      exploit (snd_forwardF_inv _ _ _ _ _ _ _ H16); eauto.
-      exploit (snd_forwardF_inv' _ _ _ _ _ _ _ H16); eauto.
-      exploit (@joinTopAnn_map_inv bool). eapply H9.
-      eapply H1; eauto.
-      * eapply (@snd_forwardF_inv_get); eauto.
-        intros. admit.
-      * erewrite (take_eta ❬s❭) at 1. eapply PIR2_app; eauto.
-        -- rewrite H. etransitivity; eauto. unfold FWt.
-           admit.
-        -- etransitivity; eauto.
-          eapply PIR2_drop.
-          eapply forwardF_PIR2; eauto.
-           ++ eapply @PIR2_length in H9. rewrite H9. eauto.
-           ++ admit.
-           ++ repeat PIR2_eq_simpl. rewrite H9. eauto.
-Qed.
- *)
-
-
-Transparent poEq.
-
-Lemma forward_if_inv (sT:stmt) D `{JoinSemiLattice D}
-      f fr ZL s t (d:VDom (occurVars sT) D) STt STs ZLIncl sa ta
-      (ANs:annotation s sa) (ANt:annotation t ta)
-      (EQ: fst (fst (forward f fr ZL ZLIncl t STt (fst (fst (forward f fr ZL ZLIncl s STs d sa))) ta)) ≣ d)
-      (disj1:disj (definedVars s) (definedVars t))
-      (disj2:disj (definedVars s ∪ definedVars t) (list_union (of_list ⊝ ZL)))
-  : (fst (fst (forward f fr ZL ZLIncl s STs d sa))) ≣ d.
-Proof.
-  hnf; intro x.
-  exploit (@forward_agree sT _ _ _ f fr ZL d (singleton x) s STs ZLIncl); eauto; dcr.
-  decide (x ∈ (definedVars s ∪ list_union (of_list ⊝ ZL))).
-  - specialize (EQ x).
-    rewrite <- EQ.
-    exploit (@forward_agree sT _ _ _ f fr ZL (fst (fst (forward f fr ZL ZLIncl s STs d sa))) (singleton x) t STt ZLIncl); eauto; dcr.
-    decide (x ∈ list_union (of_list ⊝ ZL)).
-    + assert (x ∉ definedVars t) by cset_tac.
-      eapply poLe_antisymmetric.
-      * specialize (H5 x). rewrite H5. reflexivity.
-        cset_tac.
-      * rewrite EQ. eapply H3. cset_tac.
-    + specialize (H4 x).
-      rewrite H4. reflexivity. cset_tac.
-  - symmetry.
-    eapply H2. cset_tac.
-Qed.
-
-Lemma forward_agree_ren sT D `{JoinSemiLattice D} f fr
-      ZL AE G s (ST:subTerm s sT) ra ZLIncl anr
-      (RA:renamedApart s ra) (AN:annotation s anr)
-  : agree_on poEq (G \ (snd (getAnn ra) ∪ list_union (of_list ⊝ ZL)))
-             (domenv (proj1_sig AE))
-             (domenv (proj1_sig
-                        (fst (fst (forward f fr ZL ZLIncl
-                                            s ST AE anr))))) /\
-    agree_on poLe (G \ (snd (getAnn ra)))
-             (domenv (proj1_sig AE))
-             (domenv (proj1_sig
-                        (fst (fst (forward f fr ZL ZLIncl
-                                            s ST AE anr))))).
-Proof.
-  rewrite <- renamedApart_occurVars; eauto.
-  eapply forward_agree; eauto.
-Qed.
-
-
-Lemma forward_agree_def_ren sT D `{JoinSemiLattice D} ZL AE G s f fr
-      (ST:subTerm s sT) ra ZLIncl anr pf
-  (RA:renamedApart s ra) (AN:annotation s anr)
-  : agree_on poEq (G \ (snd (getAnn ra) ∪ list_union (of_list ⊝ ZL)))
-             (domenv AE)
-             (domenv (proj1_sig
-                        (fst (fst (forward f fr
-                                            ZL ZLIncl
-                                            s ST (exist _ AE pf) anr))))).
-Proof.
-  edestruct forward_agree_ren with (AE:=exist _ AE pf); dcr; eauto.
-Qed.
-
-
-Lemma forward_agree_def sT D `{JoinSemiLattice D} ZL AE G s f fr
-      (ST:subTerm s sT) ra ZLIncl anr pf
-  (RA:renamedApart s ra) (AN:annotation s anr)
-  : agree_on poEq (G \ (definedVars s ∪ list_union (of_list ⊝ ZL)))
-             (domenv AE)
-             (domenv (proj1_sig
-                        (fst (fst (forward f fr
-                                            ZL ZLIncl
-                                            s ST (exist _ AE pf) anr))))).
-Proof.
-  edestruct forward_agree with (AE:=exist _ AE pf); dcr; eauto.
-Qed.
-
-Lemma forwardF_agree_get (sT:stmt) D `{JoinSemiLattice D} f fr
-      (F : 〔params * stmt〕)
-      (t : stmt)
-      (ZL : 〔params〕)
-      (ra : 〔ann (⦃nat⦄ * ⦃nat⦄)〕)
-      (AE AE': VDom (occurVars sT) D) BL
-      STF
-      (ZLIncl : list_union (of_list ⊝ ZL) [<=] occurVars sT)
-      (LenZL:❬ZL❭ >= ❬F❭)
-      (sa : 〔ann bool〕)
-      (ta : ann bool)  tra
-      (RAt:renamedApart t tra) (AN:annotation t ta)
-      (EQM :   (fst (fst (@forwardF sT (sTDom D) BL
-                                (forward f fr ZL ZLIncl) F
-                                sa
-                                AE'
-                                STF))) ≣ AE)
-      (STt:subTerm t sT)
-      (EQ: (fst (fst (forward f fr ZL ZLIncl t STt AE ta))) ≣ AE')
-      (Disj1:disj (snd (getAnn tra)) (list_union (of_list ⊝ ZL)))
-      (Disj2:disj (snd (getAnn tra)) (list_union (snd ⊝ getAnn ⊝ ra)))
-      (Disj3:disj (list_union (of_list ⊝ ZL)) (list_union (snd ⊝ getAnn ⊝ ra)))
-      (Disj5:disj (list_union (of_list ⊝ fst ⊝ F)) (list_union (snd ⊝ getAnn ⊝ ra)))
-      (Disj6:PairwiseDisjoint.pairwise_ne disj (defVars ⊜ F ra))
-      (Len2 : ❬F❭ = ❬ra❭)
-      (Len1 : ❬F❭ = ❬sa❭)
-      (AnnF : forall (n : nat) (s' : params * stmt) (sa' : ann bool),
-         get sa n sa' -> get F n s' -> annotation (snd s') sa')
-      (RA : forall (n : nat) (Zs : params * stmt) (a : ann (⦃nat⦄ * ⦃nat⦄)),
-          get F n Zs -> get ra n a -> renamedApart (snd Zs) a)
-      (fExt:forall (U : ⦃nat⦄) (e : exp) (a0 a' : VDom U D),
-          a0 ≣ a' -> forall b b' : bool, b ≣ b' -> f U b a0 e ≣ f U b' a' e)
-      (frExt:forall (U : ⦃nat⦄) (e : op) (a0 a' : VDom U D),
-          a0 ≣ a' -> forall b b' : bool, b ≣ b' -> fr U b a0 e ≣ fr U b' a' e)
-  : (fst (fst (forward f fr ZL ZLIncl t STt AE ta)) ≣ AE)
-    /\  forall n Zs r (ST : subTerm (snd Zs) sT),
-      get F n Zs ->
-      get sa n r ->
-      fst (fst (forward f fr ZL ZLIncl (snd Zs) ST AE r)) ≣ AE.
-Proof.
-  Opaque poEq.
-  general induction Len1; simpl in *; eauto.
-  - split; isabsurd. etransitivity; eauto.
-  - destruct ra; simpl in *; isabsurd.
-    revert Disj2 Disj3 Disj5. norm_lunion. intros Disj2 Disj3 Disj5.
-    edestruct (IHLen1 sT _ _ _ f fr t ZL); eauto using get.
-    + Transparent poEq.
-      hnf; intros z.
-      exploit (@forward_agree_ren sT _ _ _ f fr ZL AE (singleton z) t STt tra ZLIncl); eauto; dcr.
-      exploit (@forward_agree_ren sT _ _ _ f fr ZL AE' (singleton z) (snd x) (STF 0 x (getLB XL x)) a ZLIncl); eauto using get; dcr.
-      exploit (@forwardF_agree sT _ _ _ BL (singleton z) XL f fr YL ZL ZLIncl);
-      eauto using get; dcr.
-      * eauto with len.
-      * intros. inv_get. inv_get. exploit (RA (S n)); eauto using get.
-        eapply renamedApart_occurVars in H9; eauto.
-        rewrite H9.
-        eapply forward_agree_ren; eauto using get.
-      * (*
-(*    instantiate (3:=(fst (fst (forward f fr ZL ZLIncl (STF 0 x (getLB _ _)) AE' y)))) in H6.
-    instantiate (1:=(fun (n : nat) (s : params * stmt) (H : get XL n s) =>
-                     STF (S n) s (getLS x H))) in H6.*)
-    unfold domenv in *.
-    decide (z ∈ snd (getAnn tra) ∪ list_union (of_list ⊝ ZL)).
-    + eapply disj_union_inv in i. destruct i; dcr.
-      * rewrite EQ.
-        eapply H4.
-        revert H8 H9 Disj2. clear.
-        intros. cset_tac.
-      * eapply poLe_antisymmetric.
-        -- rewrite EQ.
-           eapply H5.
-           revert H8 Disj3; clear_all. intros. cset_tac.
-        -- etransitivity; [| eapply H3].
-           rewrite <- EQM.
-           eapply H7.
-           revert H8 Disj3. clear_all; intros.
-           cset_tac.
-           revert H9; clear_all; cset_tac.
-      * eapply disj_2_incl; try eapply Disj1; eauto.
-    + decide (z ∈ (list_union (defVars ⊜ XL ra))).
-      * clear H7 H6.
-        rewrite EQ. eapply H4.
-        eapply (@defVars_drop_disj (x::XL) (a::ra) 0) in Disj6;
-          eauto using get. simpl in *.
-        unfold defVars in Disj6 at 1.
-        rewrite list_union_defVars_decomp in *; eauto.
-        revert n i Disj5 Disj6. clear_all.
-        intros. cset_tac.
-      * exploit (H2 z). revert n; clear_all; cset_tac.
-        rewrite <- H1.
-        rewrite <- EQM. symmetry. eapply H6.
-        revert n n0; clear_all; cset_tac.
-    + eapply disj_2_incl; eauto.
-    + eapply disj_2_incl. eapply Disj3. clear_all; cset_tac.
-    + eapply disj_incl. eapply Disj5.
-      clear_all; cset_tac.
-      clear_all; cset_tac.
-    + hnf; intros. eapply Disj6; [|eauto using get|eauto using get]. omega.
-    + intros; split; eauto.
-      intros. inv H3; inv H4; eauto using get.
-      assert (AEQ:AE === AE').
-      { hnf; intros.
-        rewrite <- EQ. rewrite H1. reflexivity.
-      }
-      assert (EQF:@forwardF sT (sTDom D) BL (forward f fr ZL ZLIncl) XL YL
-                       (fst (fst (forward f fr ZL ZLIncl (STF 0 Zs (@getLB (params * stmt) XL Zs)) AE' r)))
-                       (fun (n : nat) (s : params * stmt) (H : get XL n s) =>
-                          STF (S n) s (getLS Zs H)) ===
-                       forwardF BL (forward f fr ZL ZLIncl) XL YL
-                       (fst (fst (forward f fr ZL ZLIncl ST AE r)))
-                       (fun (n : nat) (s : params * stmt) (H : get XL n s) =>
-                          STF (S n) s (getLS Zs H))
-             ). {
-        eapply forwardF_ext; eauto.
-        intros. eapply forward_ext; eauto.
-        assert ((STF 0 Zs (@getLB (params * stmt) XL Zs)) = ST) by eapply subTerm_PI.
-        subst.
-        eapply forward_ext; eauto.
-        symmetry; eauto.
-      }
-       hnf; intros z.
-    exploit (@forward_agree sT _ _ _ f fr ZL AE (singleton z) (snd Zs) ST a ZLIncl); eauto using get; dcr.
-    exploit (@forwardF_agree sT _ _ _  BL (singleton z) XL f fr ra YL ZL ZLIncl);
-      eauto using get; dcr.
-    eauto with len.
-    intros. inv_get.
-    eapply forward_agree; eauto using get.
-    unfold domenv in *.
-    decide (z ∈ snd (getAnn tra) ∪ list_union (of_list ⊝ ZL)).
-    * eapply disj_union_inv in i. destruct i; dcr.
-      -- symmetry.
-         eapply (H6 z).
-         revert H10 H11 Disj2. clear.
-         intros. cset_tac.
-      -- eapply poLe_antisymmetric.
-         ++ etransitivity.
-           eapply H9.
-           revert H10 Disj3; clear_all. intros. cset_tac.
-           rewrite <- EQM.
-           hnf in EQF. dcr.
-           hnf in H5. dcr.
-           specialize (H13 z).
-           rewrite H13. reflexivity.
-         ++ eapply H7.
-           revert H10 H11 Disj3; clear_all. intros. cset_tac.
-      -- eauto.
-    * decide (z ∈ (list_union (defVars ⊜ XL ra))).
-      -- symmetry.
-         eapply H6.
-         eapply (@defVars_drop_disj (Zs::XL) (a::ra) 0) in Disj6;
-           eauto using get. simpl in *.
-        unfold defVars in Disj6 at 1.
-        rewrite list_union_defVars_decomp in Disj6; eauto.
-        rewrite list_union_defVars_decomp in i; eauto.
-        revert n i Disj5 Disj6. clear_all.
-        intros. cset_tac.
-      -- rewrite (H8 z).
-         rewrite <- EQM.
-         hnf in EQF. dcr.
-         hnf in H5. dcr.
-         specialize (H11 z).
-         rewrite H11. reflexivity.
-         revert n n0; clear_all; cset_tac.
-Qed.
-         *)
-Admitted.
-Opaque poEq.
-
-
-
-Definition reachability_sound (sT:stmt) D `{JoinSemiLattice D}
-           f fr pr ZL BL s (d:VDom (occurVars sT) D) r (ST:subTerm s sT) ZLIncl
-           (EQ:(fst (forward f fr ZL ZLIncl s ST d r)) ≣ (d,r)) ra
-    (Ann: annotation s r) (RA:renamedApart s ra)
-    (DefZL: labelsDefined s (length ZL))
-    (DefBL: labelsDefined s (length BL))
-    (BL_le: poLe (snd (forward f fr ZL ZLIncl s ST d r)) BL)
-    (Disj:disj (list_union (of_list ⊝ ZL)) (snd (getAnn ra)))
-    (frIndep:forall U e (a a':VDom U D),
-        forall b b', b ≣ b' -> fr _ b a e ≣ fr _ b' a' e)
-  : reachability pr Sound BL s r.
-Proof.
-  general induction Ann; invt renamedApart; simpl in *; inv DefZL; inv DefBL;
-    repeat let_case_eq; repeat simpl_pair_eqs; subst; simpl in *;
-      simpl in *; inv_cleanup.
-  - clear_trivial_eqs.
-    econstructor; eauto.
-    eapply IHAnn; eauto. split; simpl; eauto.
-    exploit (@forward_agree sT _ _ _ f fr ZL (domupdd d (f (occurVars sT) (getAnn sa) d e) (subTerm_EQ_Let_x eq_refl ST)) (singleton x) s (subTerm_EQ_Let eq_refl ST) ZLIncl); eauto; dcr.
-    exploit (H2 x).
-    rewrite renamedApart_occurVars; eauto. pe_rewrite. set_simpl.
-    eapply renamedApart_disj in H6. pe_rewrite. revert H6 Disj.
-    clear_all. cset_tac.
-    rewrite EQ.
-    eapply domupdd_eq.
-    exploit (EQ x).
-    rewrite H7 in H1.
-    rewrite <- H1. symmetry.
-    unfold domenv, domupdd; simpl.
-    rewrite domupd_var_eq. reflexivity. reflexivity.
-    pe_rewrite. eapply disj_2_incl; eauto. cset_tac.
-  - clear_trivial_eqs.
-    set_simpl.
-    econstructor; eauto.
-    + admit.
-    + admit.
-    + eapply IHAnn1;
-        eauto using @PIR2_zip_join_inv_left, @PIR2_zip_join_inv_right with len.
-      * split; simpl; eauto.
-        eapply forward_if_inv; eauto;
-          repeat rewrite renamedApart_occurVars; eauto;
-            pe_rewrite; eauto with cset.
-      * pe_rewrite. eapply disj_2_incl; eauto.
-    + eapply IHAnn2;
-        eauto using @PIR2_zip_join_inv_left, @PIR2_zip_join_inv_right with len.
-      * split; simpl; eauto.
-        rewrite EQ. symmetry.
-        eapply forward_if_inv; eauto;
-          repeat rewrite renamedApart_occurVars; eauto;
-            pe_rewrite; eauto with cset.
-      * pe_rewrite. eapply disj_2_incl; eauto.
-  - edestruct get_in_range; eauto.
-    edestruct get_in_range; try eapply H7; eauto.
-    Transparent poLe. hnf in BL_le.
+    Transparent poLe. hnf in H.
     edestruct PIR2_nth; eauto using ListUpdateAt.list_update_at_get_3; dcr.
     econstructor; simpl; eauto.
   - econstructor.
-  - clear_trivial_eqs.
-    set (FWt:=(forward f fr (fst ⊝ s ++ ZL) (ZLIncl_ext ZL eq_refl ST ZLIncl) t
-                       (subTerm_EQ_Fun1 eq_refl ST) d ta)) in *.
-    set (FWF:=forwardF (snd FWt) (forward f fr (fst ⊝ s ++ ZL) (ZLIncl_ext ZL eq_refl ST ZLIncl)) s (joinTopAnn (A:=bool) ⊜ sa (snd FWt)) (fst (fst FWt)) (subTerm_EQ_Fun2 eq_refl ST)) in *.
+  - invc EQ. simpl_forward_setTopAnn.
+    revert H2 H16 H16 H15.
+    set (FWt:=(forward reachability_transform (fst ⊝ s ++ ZL) t
+                       (subTerm_EQ_Fun1 eq_refl ST) (getAnn ta) ta)).
+    set (FWF:=forwardF (forward reachability_transform) (fst ⊝ s ++ ZL) s sa
+                       (subTerm_EQ_Fun2 eq_refl ST)).
     intros.
-    eapply PIR2_get in H23; eauto with len.
-    exploit (snd_forwardF_inv _ _ _ _ _ _ _ H23); eauto.
-    subst FWt. len_simpl. omega.
-    subst FWt. len_simpl. omega.
-    exploit (snd_forwardF_inv' _ _ _ _ _ _ _ H23); eauto.
-    subst FWt. len_simpl. omega.
-    subst FWt. len_simpl. omega.
-    assert (forall (n : nat) (r : ann bool) (Zs : params * stmt),
-       get sa n r ->
-       get s n Zs ->
-       forall STZs : subTerm (snd Zs) sT,
-       ann_R eq
-         (snd
-            (fst
-               (forward f fr (fst ⊝ s ++ ZL) (ZLIncl_ext ZL eq_refl ST ZLIncl)
-                        (snd Zs) STZs (fst (fst FWt)) r))) r).
-    eapply (@snd_forwardF_inv_get); eauto.
-    subst FWt. len_simpl.  omega.
-    subst FWt. len_simpl. omega.
-    intros. admit. admit.
-    Transparent poEq.
-    repeat PIR2_eq_simpl.
-    subst FWF FWt.
-    rewrite H23 in *.
-    rewrite H4 in *.
-    rewrite H5 in *.
-    set (FWt:=(forward f fr (fst ⊝ s ++ ZL) (ZLIncl_ext ZL eq_refl ST ZLIncl) t
-                       (subTerm_EQ_Fun1 eq_refl ST) d ta)) in *.
-    set (FWF:=forwardF (snd FWt) (forward f fr (fst ⊝ s ++ ZL) (ZLIncl_ext ZL eq_refl ST ZLIncl)) s sa (fst (fst FWt)) (subTerm_EQ_Fun2 eq_refl ST)) in *.
-    Opaque poEq. inv_cleanup.
-
     econstructor; eauto.
     + eapply IHAnn; eauto.
-      * split; eauto. simpl.
-        admit.
-      * erewrite (take_eta ❬s❭) at 1. eapply PIR2_app; eauto.
-        --change (PIR2 poLe) with (@poLe (list bool) _).
-           assert (poLe (Take.take ❬s❭ (snd FWt)) (getAnn ⊝ sa)). {
-             rewrite H.
-             eapply (@joinTopAnn_map_inv).
-             rewrite <- H4 at 2. reflexivity.
-           }
-           rewrite <- H4. subst FWF.
-           subst FWt.
-           rewrite H4.
-           rewrite <- H5.
-           rewrite <- (@forwardF_mon' sT D _ _ f fr); eauto.
-        -- rewrite <- BL_le.
-           eapply PIR2_drop.
-           etransitivity;[|
-                          eapply forwardF_mon; eauto].
-           reflexivity.
-           subst FWt. eauto with len.
-      * pe_rewrite.
-        admit.
-    + intros. inv_get. exploit H7; eauto.
-      eapply H1; eauto.
-      -- subst FWF FWt.
+      erewrite (take_eta ❬s❭) at 1. eapply PIR2_app; eauto.
+      * eapply PIR2_get; eauto with len. intros. inv_get.
+        edestruct (get_forwardF (fun _ => bool) (forward reachability_transform)
+                                (fst ⊝ s ++ ZL) (subTerm_EQ_Fun2 eq_refl ST) H11 H8).
+        edestruct (@get_union_union_b bool _ _).
+        eapply H4; eauto with len.
+        Focus 2. dcr.
+        exploit H15. eapply zip_get. eapply map_get_1; eauto.
+        eapply H12. eauto. eapply ann_R_get in H3. rewrite <- H3.
+        rewrite getAnn_setTopAnn. eauto.
+        intros. inv_get.
+        edestruct (@forwardF_get _ _ _ _ _ _ _ _ _ _ _ H3); dcr; subst;
+          eauto with len.
+      * etransitivity; eauto. eapply PIR2_drop.
+        eapply PIR2_fold_zip_join_inv. reflexivity.
+        intros.
+        inv_get.
+        edestruct (@forwardF_get _ _ _ _ _ _ _ _ _ _ _ H4). dcr. subst.
+        eauto with len.
+    + intros.
+      assert (n < ❬snd FWt❭). {
+        subst FWt.
+        repeat rewrite (@forward_length sT (fun _ => bool)). rewrite app_length. rewrite map_length.
+        eapply get_range in H8. omega.
+      }
+      edestruct get_in_range; eauto.
+      edestruct (get_forwardF (fun _ => bool) (forward reachability_transform)
+                              (fst ⊝ s ++ ZL) (subTerm_EQ_Fun2 eq_refl ST) H4 H8).
+      eapply H1 with (ST:=x0); eauto.
+      eapply H15; eauto.
+      *
+        assert (n <
+                ❬snd (
+                     forward reachability_transform (fst ⊝ s ++ ZL) (snd Zs) x0 (getAnn a) a)❭). {
+          erewrite (@forward_length sT (fun _ => bool)). rewrite app_length,map_length.
+          eapply get_range in H8. omega.
+        }
+        edestruct get_in_range; eauto.
+        exploit (@get_union_union_A bool _ _).
+        eapply map_get_1. apply g0. instantiate (3:=snd). eauto.
+        Focus 2.
+        destruct H12; dcr.
+        eapply zip_get_eq. eapply map_get_1. eauto.  eauto.
+        exploit H15.
+        eapply zip_get.
+        eapply map_get_1. eauto. eapply H13. eauto.
+        exploit (setTopAnn_inv _ _ H12); eauto; subst.
+        rewrite setTopAnn_eta; eauto.
+        eapply (@forward_getAnn' sT (fun _ => bool)).
 
-         exploit  forwardF_agree_get; eauto.
-         len_simpl. omega.
+        clear_all. intros. inv_get.
+        subst FWt.
+        len_simpl. eauto with len.
 
-        split; simpl; eauto. simpl. reflexivity.
-      -- rewrite (take_eta ❬sa❭) at 1.
-         eapply PIR2_app; eauto.
-         ++ eapply setTopAnn_map_inv in H15.
-           rewrite <- H15. eapply PIR2_take.
-           change (PIR2 impb) with (@poLe (list bool) _).
-           eapply forwardF_PIR2; eauto.
-           subst FWt. clear_all. eauto with len.
-
-         ++ etransitivity; eauto.
-           rewrite H. eapply PIR2_drop.
-           eapply forwardF_PIR2; eauto.
-           subst FWt. eauto with len.
-           admit.
+      * rewrite (take_eta ❬sa❭) at 1.
+        eapply PIR2_app.
+        protect g0.
+        eapply PIR2_get; intros; inv_get.
+        exploit (@get_union_union_A bool _ _).
+        eapply map_get_1. apply g0. instantiate (3:=snd). eauto.
+        Focus 2. dcr.
+        edestruct (get_forwardF (fun _ => bool) (forward reachability_transform)
+                                (fst ⊝ s ++ ZL) (subTerm_EQ_Fun2 eq_refl ST) H17 H12).
+        exploit H15; eauto.
+        eapply zip_get. eapply map_get_1. subst FWF. eauto. eauto.
+        eapply ann_R_get in H3. rewrite getAnn_setTopAnn in H3. rewrite <- H3.
+        eauto.
+        clear_all. intros. inv_get.
+        subst FWt. eauto with len.
+        rewrite Take.take_length_le; eauto with len.
+        etransitivity; eauto.
+        rewrite H. eapply PIR2_drop.
+        subst FWF.
+        pose proof (@PIR2_fold_zip_join_left bool _ _). eapply H11.
+        eauto. reflexivity.
+        clear_all. intros. inv_get.
+        subst FWt. eauto with len.
 Qed.
 
 Lemma impl_poLe (a b:bool)
@@ -844,7 +399,7 @@ Proof.
       eapply H2. eauto. rewrite setTopAnn_eta. eauto.
       eauto.
       eauto with len.
-      eauto.
+      eauto. Transparent poLe.
       eapply ann_R_get in H8. rewrite getAnn_setTopAnn in H8.
       eauto.
       etransitivity; eauto.
